more tests of Move `AbstractStack` methods

CoqOfRust/move_sui/simulations/move_abstract_stack/unit_tests/mod.v
@@ -55,3 +55,287 @@ Lemma test_empty_stack_correct :
 Proof.
   reflexivity.
 Qed.
+
+(*
+  #[test]
+  fn test_simple_push_pop() {
+      let mut s = AbstractStack::new();
+      s.push(1).unwrap();
+      assert!(!s.is_empty());
+      assert_eq!(s.len(), 1);
+      s.assert_run_lengths([1]);
+      assert_eq!(s.pop(), Ok(1));
+      assert!(s.is_empty());
+      assert_eq!(s.len(), 0);
+
+      s.push(1).unwrap();
+      s.push(2).unwrap();
+      s.push(3).unwrap();
+      assert!(!s.is_empty());
+      assert_eq!(s.len(), 3);
+      s.assert_run_lengths([1, 1, 1]);
+      assert_eq!(s.pop(), Ok(3));
+      assert_eq!(s.pop(), Ok(2));
+      assert_eq!(s.pop(), Ok(1));
+      assert!(s.is_empty());
+      assert_eq!(s.len(), 0);
+
+      s.push_n(1, 1).unwrap();
+      s.push_n(2, 2).unwrap();
+      s.push_n(3, 3).unwrap();
+      assert!(!s.is_empty());
+      assert_eq!(s.len(), 6);
+      s.assert_run_lengths([1, 2, 3]);
+      assert_eq!(s.pop(), Ok(3));
+      assert_eq!(s.pop(), Ok(3));
+      assert_eq!(s.pop(), Ok(3));
+      assert_eq!(s.pop(), Ok(2));
+      assert_eq!(s.pop(), Ok(2));
+      assert_eq!(s.pop(), Ok(1));
+      assert!(s.is_empty());
+      assert_eq!(s.len(), 0);
+
+      s.push_n(1, 1).unwrap();
+      s.push_n(2, 2).unwrap();
+      s.push_n(3, 3).unwrap();
+      assert!(!s.is_empty());
+      assert_eq!(s.len(), 6);
+      s.assert_run_lengths([1, 2, 3]);
+      assert_eq!(s.pop_eq_n(nonzero(3)), Ok(3));
+      assert_eq!(s.pop_eq_n(nonzero(2)), Ok(2));
+      assert_eq!(s.pop_eq_n(nonzero(1)), Ok(1));
+      assert!(s.is_empty());
+      assert_eq!(s.len(), 0);
+
+      s.push(1).unwrap();
+      s.push(2).unwrap();
+      s.push(2).unwrap();
+      s.push(3).unwrap();
+      s.push(3).unwrap();
+      s.push(3).unwrap();
+      assert!(!s.is_empty());
+      s.assert_run_lengths([1, 2, 3]);
+      assert_eq!(s.len(), 6);
+      assert_eq!(s.pop_eq_n(nonzero(3)), Ok(3));
+      assert_eq!(s.pop_eq_n(nonzero(2)), Ok(2));
+      assert_eq!(s.pop_eq_n(nonzero(1)), Ok(1));
+      assert!(s.is_empty());
+      assert_eq!(s.len(), 0);
+
+      s.push_n(1, 1).unwrap();
+      s.push_n(2, 2).unwrap();
+      s.push_n(3, 3).unwrap();
+      assert!(!s.is_empty());
+      s.assert_run_lengths([1, 2, 3]);
+      assert_eq!(s.len(), 6);
+      s.pop_any_n(nonzero(6)).unwrap();
+      assert_eq!(s.len(), 0);
+      assert!(s.is_empty());
+
+      s.push(1).unwrap();
+      s.push(2).unwrap();
+      s.push(2).unwrap();
+      s.push(3).unwrap();
+      s.push(3).unwrap();
+      s.push(3).unwrap();
+      assert!(!s.is_empty());
+      s.assert_run_lengths([1, 2, 3]);
+      assert_eq!(s.len(), 6);
+      s.pop_any_n(nonzero(4)).unwrap();
+      s.pop_any_n(nonzero(2)).unwrap();
+      assert!(s.is_empty());
+      assert_eq!(s.len(), 0);
+  }
+*)
+
+Definition test_simple_push_pop :
+    MS? (AbstractStack.t Z) string unit :=
+
+  letS? s := readS? in
+  letS? _ := AbstractStack.push 1 in
+  letS? _ := assertS?ofS? AbstractStack.self_is_not_empty in
+  letS? _ := assert_eqS?ofS? AbstractStack.self_len (returnS? 1) in
+  letS? _ := AbstractStack.assert_run_lengths [1] in
+  letS? _ := assert_eqS?ofS? AbstractStack.pop (returnS? (Result.Ok 1)) in
+  letS? _ := assertS?ofS? (AbstractStack.self_is_empty) in
+  letS? _ := assert_eqS?ofS? AbstractStack.self_len (returnS? 0) in
+
+  letS? _ := AbstractStack.push 1 in
+  letS? _ := AbstractStack.push 2 in
+  letS? _ := AbstractStack.push 3 in
+  letS? _ := assertS?ofS? AbstractStack.self_is_not_empty in
+  letS? _ := assert_eqS?ofS? AbstractStack.self_len (returnS? 3) in
+  letS? _ := AbstractStack.assert_run_lengths [1; 1; 1] in
+  letS? _ := assert_eqS?ofS? AbstractStack.pop (returnS? (Result.Ok 3)) in
+  letS? _ := assert_eqS?ofS? AbstractStack.pop (returnS? (Result.Ok 2)) in
+  letS? _ := assert_eqS?ofS? AbstractStack.pop (returnS? (Result.Ok 1)) in
+  letS? _ := assertS?ofS? (AbstractStack.self_is_empty) in
+  letS? _ := assert_eqS?ofS? AbstractStack.self_len (returnS? 0) in
+
+  letS? _ := AbstractStack.push_n 1 1 in
+  letS? _ := AbstractStack.push_n 2 2 in
+  letS? _ := AbstractStack.push_n 3 3 in
+  letS? _ := assertS?ofS? AbstractStack.self_is_not_empty in
+  letS? _ := assert_eqS?ofS? AbstractStack.self_len (returnS? 6) in
+  letS? _ := AbstractStack.assert_run_lengths [3; 2; 1] in
+  letS? _ := assert_eqS?ofS? AbstractStack.pop (returnS? (Result.Ok 3)) in
+  letS? _ := assert_eqS?ofS? AbstractStack.pop (returnS? (Result.Ok 3)) in
+  letS? _ := assert_eqS?ofS? AbstractStack.pop (returnS? (Result.Ok 3)) in
+  letS? _ := assert_eqS?ofS? AbstractStack.pop (returnS? (Result.Ok 2)) in
+  letS? _ := assert_eqS?ofS? AbstractStack.pop (returnS? (Result.Ok 2)) in
+  letS? _ := assert_eqS?ofS? AbstractStack.pop (returnS? (Result.Ok 1)) in
+  letS? _ := assertS?ofS? (AbstractStack.self_is_empty) in
+  letS? _ := assert_eqS?ofS? AbstractStack.self_len (returnS? 0) in
+
+  letS? _ := AbstractStack.push_n 1 1 in
+  letS? _ := AbstractStack.push_n 2 2 in
+  letS? _ := AbstractStack.push_n 3 3 in
+  letS? _ := assertS?ofS? AbstractStack.self_is_not_empty in
+  letS? _ := assert_eqS?ofS? AbstractStack.self_len (returnS? 6) in
+  letS? _ := AbstractStack.assert_run_lengths [3; 2; 1] in
+  letS? _ := assert_eqS?ofS? (AbstractStack.pop_eq_n 3) (returnS? (Result.Ok 3)) in
+  letS? _ := assert_eqS?ofS? (AbstractStack.pop_eq_n 2) (returnS? (Result.Ok 2)) in
+  letS? _ := assert_eqS?ofS? (AbstractStack.pop_eq_n 1) (returnS? (Result.Ok 1)) in
+  letS? _ := assertS?ofS? (AbstractStack.self_is_empty) in
+  letS? _ := assert_eqS?ofS? AbstractStack.self_len (returnS? 0) in
+
+  letS? _ := AbstractStack.push 1 in
+  letS? _ := AbstractStack.push 2 in
+  letS? _ := AbstractStack.push 2 in
+  letS? _ := AbstractStack.push 3 in
+  letS? _ := AbstractStack.push 3 in
+  letS? _ := AbstractStack.push 3 in
+  letS? _ := assertS?ofS? AbstractStack.self_is_not_empty in
+  letS? _ := AbstractStack.assert_run_lengths [3; 2; 1] in
+  letS? _ := assert_eqS?ofS? AbstractStack.self_len (returnS? 6) in
+  letS? _ := assert_eqS?ofS? (AbstractStack.pop_eq_n 3) (returnS? (Result.Ok 3)) in
+  letS? _ := assert_eqS?ofS? (AbstractStack.pop_eq_n 2) (returnS? (Result.Ok 2)) in
+  letS? _ := assert_eqS?ofS? (AbstractStack.pop_eq_n 1) (returnS? (Result.Ok 1)) in
+  letS? _ := assertS?ofS? (AbstractStack.self_is_empty) in
+  letS? _ := assert_eqS?ofS? AbstractStack.self_len (returnS? 0) in
+
+  letS? _ := AbstractStack.push_n 1 1 in
+  letS? _ := AbstractStack.push_n 2 2 in
+  letS? _ := AbstractStack.push_n 3 3 in
+  letS? _ := assertS?ofS? AbstractStack.self_is_not_empty in
+  letS? _ := AbstractStack.assert_run_lengths [3; 2; 1] in
+  letS? _ := assert_eqS?ofS? AbstractStack.self_len (returnS? 6) in
+  letS? _ := AbstractStack.pop_any_n 6 in
+  letS? _ := assert_eqS?ofS? AbstractStack.self_len (returnS? 0) in
+  letS? _ := assertS?ofS? (AbstractStack.self_is_empty) in
+
+  letS? _ := AbstractStack.push 1 in
+  letS? _ := AbstractStack.push 2 in
+  letS? _ := AbstractStack.push 2 in
+  letS? _ := AbstractStack.push 3 in
+  letS? _ := AbstractStack.push 3 in
+  letS? _ := AbstractStack.push 3 in
+  letS? _ := assertS?ofS? AbstractStack.self_is_not_empty in
+  letS? _ := AbstractStack.assert_run_lengths [3; 2; 1] in
+  letS? _ := assert_eqS?ofS? AbstractStack.self_len (returnS? 6) in
+  letS? _ := AbstractStack.pop_any_n 4 in
+  letS? _ := AbstractStack.pop_any_n 2 in
+  letS? _ := assertS?ofS? (AbstractStack.self_is_empty) in
+  letS? _ := assert_eqS?ofS? AbstractStack.self_len (returnS? 0) in
+
+  returnS? tt.
+
+Lemma test_simple_push_pop_correct :
+  testS? test_simple_push_pop AbstractStack.new.
+Proof.
+  reflexivity.
+Qed.
+
+(*
+  #[test]
+  fn test_not_eq() {
+      let mut s = AbstractStack::new();
+      s.push(1).unwrap();
+      s.push(2).unwrap();
+      s.push(2).unwrap();
+      s.push(3).unwrap();
+      s.push(3).unwrap();
+      s.push(3).unwrap();
+      assert_eq!(s.len(), 6);
+      s.assert_run_lengths([1, 2, 3]);
+      assert_eq!(s.pop_eq_n(nonzero(4)), Err(AbsStackError::ElementNotEqual));
+      assert_eq!(s.pop_eq_n(nonzero(5)), Err(AbsStackError::ElementNotEqual));
+      assert_eq!(s.len(), 6);
+      s.assert_run_lengths([1, 2, 3]);
+  }
+*)
+
+Definition test_not_eq :
+    MS? (AbstractStack.t Z) string unit :=
+  letS? s := readS? in
+  letS? _ := AbstractStack.push 1 in
+  letS? _ := AbstractStack.push 2 in
+  letS? _ := AbstractStack.push 2 in
+  letS? _ := AbstractStack.push 3 in
+  letS? _ := AbstractStack.push 3 in
+  letS? _ := AbstractStack.push 3 in
+  letS? _ := assert_eqS?ofS? AbstractStack.self_len (returnS? 6) in
+  letS? _ := AbstractStack.assert_run_lengths [3; 2; 1] in
+  letS? _ :=
+    assert_eqS?ofS?
+      (AbstractStack.pop_eq_n 4)
+      (returnS? (Result.Err AbsStackError.ElementNotEqual)) in
+  letS? _ :=
+    assert_eqS?ofS?
+      (AbstractStack.pop_eq_n 4)
+      (returnS? (Result.Err AbsStackError.ElementNotEqual)) in
+  letS? _ := assert_eqS?ofS? (AbstractStack.self_len) (returnS? 6) in
+  AbstractStack.assert_run_lengths [3; 2; 1].
+
+Lemma test_not_eq_correct :
+  testS? test_not_eq AbstractStack.new.
+Proof.
+  reflexivity.
+Qed.
+
+(*
+  #[test]
+  fn test_not_enough_values() {
+      let mut s = AbstractStack::new();
+      s.push(1).unwrap();
+      s.push(2).unwrap();
+      s.push(2).unwrap();
+      s.push(3).unwrap();
+      s.push(3).unwrap();
+      s.push(3).unwrap();
+      assert_eq!(s.len(), 6);
+      s.assert_run_lengths([1, 2, 3]);
+      assert_eq!(s.pop_eq_n(nonzero(7)), Err(AbsStackError::Underflow));
+      assert_eq!(s.pop_any_n(nonzero(7)), Err(AbsStackError::Underflow));
+      assert_eq!(s.len(), 6);
+      s.assert_run_lengths([1, 2, 3]);
+  }
+*)
+
+Definition test_not_enough_values :
+    MS? (AbstractStack.t Z) string unit :=
+  letS? s := readS? in
+  letS? _ := AbstractStack.push 1 in
+  letS? _ := AbstractStack.push 2 in
+  letS? _ := AbstractStack.push 2 in
+  letS? _ := AbstractStack.push 3 in
+  letS? _ := AbstractStack.push 3 in
+  letS? _ := AbstractStack.push 3 in
+  letS? _ := assert_eqS?ofS? AbstractStack.self_len (returnS? 6) in
+  letS? _ := AbstractStack.assert_run_lengths [3; 2; 1] in
+  letS? _ :=
+    assert_eqS?ofS?
+      (AbstractStack.pop_eq_n 7)
+      (returnS? (Result.Err AbsStackError.Underflow)) in
+  letS? _ :=
+    assert_eqS?ofS?
+      (AbstractStack.pop_any_n 7)
+      (returnS? (Result.Err AbsStackError.Underflow)) in
+  letS? _ := assert_eqS?ofS? (AbstractStack.self_len) (returnS? 6) in
+  AbstractStack.assert_run_lengths [3; 2; 1].
+
+Lemma test_not_enough_values_correct :
+  testS? test_not_enough_values AbstractStack.new.
+Proof.
+  reflexivity.
+Qed.
